feat(Modal): Modal Disjunctive Property of `𝐆𝐋` (#106)
* wip

* refactor

* complete

Logic/Modal/Standard/Kripke/GL/Tree.lean
@@ -1,345 +1,10 @@
-import Mathlib.Data.Fintype.List
-import Logic.Vorspiel.BinaryRelations
-import Logic.Modal.Standard.Kripke.Soundness
-import Logic.Modal.Standard.Kripke.Filteration
-import Logic.Modal.Standard.Kripke.Preservation
-
-namespace LO.Modal.Standard
-
-namespace Kripke
-
-open System
-open Kripke
-open Formula
-
-variable {α : Type u} [Inhabited α]
-
-section Definability_and_Soundness
-
-variable {F : Kripke.Frame}
-
-abbrev TransitiveCWFFrameClass : FrameClass := { F | Transitive F ∧ ConverseWellFounded F }
-
-private lemma trans_of_L : F# ⊧* (𝗟 : AxiomSet α) → Transitive F.Rel := by
-  contrapose;
-  intro hT; simp [Transitive] at hT;
-  obtain ⟨w₁, w₂, r₁₂, w₃, r₂₃, nr₁₃⟩ := hT;
-  apply iff_not_validOnFrame.mpr;
-  use (Axioms.L (atom default));
-  constructor;
-  . simp;
-  . use (λ w' _ => w' ≠ w₂ ∧ w' ≠ w₃), w₁;
-    simp only [Kripke.Satisfies]; push_neg;
-    constructor;
-    . intro x hx h;
-      by_cases hx₂ : x = w₂;
-      . subst hx₂; simpa [Kripke.Satisfies] using h r₂₃;
-      . by_cases hx₃ : x = w₃ <;> simp_all [Kripke.Satisfies, hx₃];
-    . existsi w₂; simpa [Kripke.Satisfies];
-
-private lemma cwf_of_L  : F# ⊧* (𝗟 : AxiomSet α) → ConverseWellFounded F.Rel := by
-  contrapose;
-  intro hCF;
-  obtain ⟨X, hX₁, hX₂⟩ := by simpa using ConverseWellFounded.iff_has_max.not.mp hCF;
-  apply iff_not_validOnFrame.mpr;
-  use (Axioms.L (atom default));
-  constructor;
-  . simp;
-  . use (λ w _ => w ∉ X), hX₁.some;
-    simp only [Kripke.Satisfies]; push_neg;
-    constructor;
-    . intro x _;
-      by_cases hxs : x ∈ X
-      . obtain ⟨y, hy₁, hy₂⟩ := hX₂ x hxs;
-        intro h;
-        exact h (by simp_all only [Kripke.Satisfies]);
-      . aesop;
-    . obtain ⟨w', hw'₁, hw'₂⟩ := hX₂ hX₁.some (by apply Set.Nonempty.some_mem);
-      existsi w';
-      constructor;
-      . simpa using hw'₂;
-      . simpa [Kripke.Satisfies];
-
-private lemma L_of_trans_and_cwf : (Transitive F.Rel ∧ ConverseWellFounded F.Rel) → F# ⊧* (𝗟 : AxiomSet α) := by
-  rintro ⟨hTrans, hWF⟩;
-  simp [Axioms.L];
-  intro p V w;
-  simp only [Kripke.Satisfies.iff_models, Kripke.Satisfies];
-  contrapose; push_neg;
-  intro h;
-  obtain ⟨z, rwz, hz⟩ := h;
-  obtain ⟨m, ⟨⟨rwm, hm⟩, hm₂⟩⟩ := hWF.has_min ({ x | (F.Rel w x) ∧ ¬(Kripke.Satisfies ⟨F, V⟩ x p) }) (by use z; simp_all)
-  use m;
-  constructor;
-  . exact rwm;
-  . constructor;
-    . simp [flip] at hm₂;
-      intro n rmn;
-      apply not_imp_not.mp $ hm₂ n (hTrans rwm rmn);
-      exact rmn;
-    . exact hm;
-
-lemma axiomL_defines : AxiomSet.DefinesKripkeFrameClass (α := α) 𝗟 (TransitiveCWFFrameClass) := by
-  intro F;
-  constructor;
-  . intro h;
-    constructor;
-    . exact trans_of_L h;
-    . exact cwf_of_L h;
-  . exact L_of_trans_and_cwf;
-
-
-abbrev TransitiveIrreflexiveFrameClass : FrameClass := { F | Transitive F ∧ Irreflexive F }
-
-/-
-lemma TransitiveIrreflexiveFiniteFrameClass.nonempty : TransitiveIrreflexiveFrameClass.Nonempty.{0} := by
-  use PointFrame;
-  simp [Transitive, Irreflexive];
--/
-
-lemma axiomL_finite_defines : AxiomSet.FinitelyDefinesKripkeFrameClass (α := α) 𝗟 ↑TransitiveIrreflexiveFrameClass := by
-  intro F;
-  constructor;
-  . intro h;
-    obtain ⟨hTrans, hCWF⟩ := axiomL_defines.mp h;
-    refine ⟨hTrans, ?irreflexive⟩;
-    . intro w;
-      simpa using ConverseWellFounded.iff_has_max.mp hCWF {w} (by simp);
-  . intro d;
-    have ⟨hTrans, hIrrefl⟩ := d;
-    apply axiomL_defines.mpr;
-    constructor;
-    . exact hTrans;
-    . exact Finite.converseWellFounded_of_trans_irrefl' F.World_finite hTrans hIrrefl;
-
-instance GL_sound : Sound (𝐆𝐋 : DeductionParameter α) TransitiveIrreflexiveFrameClassꟳ# := sound_of_finitely_defines axiomL_finite_defines
-
-instance : System.Consistent (𝐆𝐋 : DeductionParameter α) := consistent_of_finitely_defines.{u} axiomL_finite_defines $ by
-  use PointFrame;
-  simp [Transitive, Irreflexive];
-
-end Definability_and_Soundness
-
-
-section Completeness
-
-open Formula (atom)
-open Formula.Kripke
-open MaximalConsistentTheory
-
-variable [DecidableEq α]
-
-noncomputable abbrev GLCanonicalFrame := CanonicalFrame (α := α) 𝐆𝐋
-
-noncomputable abbrev GLCanonicalModel := CanonicalModel (α := α) 𝐆𝐋
-
-lemma filter_truthlemma
-  [Inhabited (Λ)-MCT] [Λ.IsNormal]
-  {T : Theory α} [T.SubformulaClosed]
-  {X Y : (CanonicalModel Λ).World} (hXY : filterEquiv _ T X Y := by aesop)
-  {p : Formula α} (hp : p ∈ T := by aesop) : p ∈ X.theory ↔ p ∈ Y.theory := by
-  constructor;
-  . intro h; exact truthlemma.mp $ hXY p hp |>.mp $ truthlemma.mpr h;
-  . intro h; exact truthlemma.mp $ hXY p hp |>.mpr $ truthlemma.mpr h;
-
-noncomputable abbrev GLFilteredFrame (p : Formula α) : Kripke.FiniteFrame where
-  World := FilterEqvQuotient GLCanonicalModel ((𝒮 p).toSet)
-  World_finite := by apply FilterEqvQuotient.finite; simp;
-  Rel := Quotient.lift₂
-    (λ X Y =>
-      (∀ q ∈ □''⁻¹(𝒮 p), □q ∈ X.theory → q ⋏ □q ∈ Y.theory) ∧
-      (∃ r ∈ □''⁻¹(𝒮 p), □r ∉ X.theory ∧ □r ∈ Y.theory)
-    )
-    (by
-      intro X₁ Y₁ X₂ Y₂ hX hY; simp;
-      constructor;
-      . rintro ⟨h₁, ⟨r, br_mem_sub, br_nmem_X₁, br_mem_Y₁⟩⟩;
-        constructor;
-        . intro q bq_mem_sub bq_mem_X₂;
-          have bq_mem_X₁ : □q ∈ X₁.theory := filter_truthlemma (by simpa) |>.mpr bq_mem_X₂;
-          have ⟨q_mem_Y₁, bq_mem_Y₁⟩ := h₁ q bq_mem_sub bq_mem_X₁;
-          constructor;
-          . exact filter_truthlemma (by simpa) |>.mp q_mem_Y₁;
-          . exact filter_truthlemma (by simpa) |>.mp bq_mem_Y₁;
-        . use r;
-          refine ⟨br_mem_sub, ?br_nmem_X₂, ?br_mem_Y₂⟩;
-          . exact filter_truthlemma (by simpa) |>.not.mp br_nmem_X₁;
-          . exact filter_truthlemma (by simpa) |>.mp br_mem_Y₁;
-      . rintro ⟨h₁, ⟨r, br_mem_sub, br_nmem_X₂, br_mem_Y₂⟩⟩;
-        constructor;
-        . intro q bq_mem_sub bq_mem_X₂;
-          have bq_mem_X₂ : □q ∈ X₂.theory := filter_truthlemma (by simpa) |>.mp bq_mem_X₂;
-          have ⟨q_mem_Y₂, bq_mem_Y₂⟩ := h₁ q bq_mem_sub bq_mem_X₂;
-          constructor;
-          . exact filter_truthlemma (by simpa) |>.mpr q_mem_Y₂;
-          . exact filter_truthlemma (by simpa) |>.mpr bq_mem_Y₂;
-        . use r;
-          refine ⟨br_mem_sub, ?m, ?me⟩;
-          . exact filter_truthlemma (by simpa) |>.not.mpr br_nmem_X₂;
-          . exact filter_truthlemma (by simpa) |>.mpr br_mem_Y₂;
-    )
-
-lemma GLFilteredFrame.def_rel {p : Formula α} {X Y : GLCanonicalFrame.World} :
-  ((GLFilteredFrame p).Rel ⟦X⟧ ⟦Y⟧) ↔
-  (∀ q ∈ □''⁻¹(𝒮 p), □q ∈ X.theory → q ⋏ □q ∈ Y.theory) ∧
-  (∃ r ∈ □''⁻¹(𝒮 p), □r ∉ X.theory ∧ □r ∈ Y.theory) := by
-  simp;
-
-noncomputable abbrev GLFilteredModel (p : Formula α) : Kripke.Model α where
-  Frame := GLFilteredFrame p
-  Valuation := StandardFilterationValuation GLCanonicalModel ((𝒮 p).toSet)
-
-variable {T : Theory α} [T.SubformulaClosed]
-variable {p : Formula α}
-
-lemma irreflexive_GLFilteredFrame : Irreflexive (GLFilteredFrame p).Rel := by
-  intro QX;
-  obtain ⟨X, hX⟩ := Quotient.exists_rep QX; subst hX;
-  simp_all;
-
-lemma transitive_GLFilteredFrame : Transitive (GLFilteredFrame p).Rel := by
-  intro QX QY QZ hXY hYZ;
-  obtain ⟨X, hX⟩ := Quotient.exists_rep QX; subst hX;
-  obtain ⟨Y, hY⟩ := Quotient.exists_rep QY; subst hY;
-  obtain ⟨Z, hZ⟩ := Quotient.exists_rep QZ; subst hZ;
-  have ⟨hXY₁, hXY₂⟩ := hXY;
-  have ⟨hYZ₁, _⟩ := hYZ;
-  constructor;
-  . intro q hq bq_mem_X;
-    have ⟨_, bq_mem_Y⟩ := MaximalConsistentTheory.iff_mem_and.mp $ hXY₁ q hq bq_mem_X;
-    exact hYZ₁ q hq bq_mem_Y;
-  . obtain ⟨r, hr, br_nmem_X, br_mem_Y⟩ := hXY₂;
-    use r;
-    constructor;
-    . assumption;
-    . constructor;
-      . assumption;
-      . have ⟨_, bq_mem_Y⟩ := MaximalConsistentTheory.iff_mem_and.mp $ hYZ₁ r hr br_mem_Y;
-        assumption;
-
-open System System.FiniteContext in
-private lemma GL_truthlemma.lemma1
-  {q : Formula α}
-  {X : (CanonicalModel 𝐆𝐋).World} (h : □q ∉ X.theory) : (𝐆𝐋)-Consistent ({□q, ~q} ∪ (□''⁻¹X.theory ∪ □''□''⁻¹X.theory)) := by
-  by_contra hC;
-  obtain ⟨Γ, hΓ₁, hΓ₂⟩ := Context.provable_iff.mp hC;
-  have := toₛ! hΓ₂;
-  have : 𝐆𝐋 ⊢! ⋀(Γ.remove (~q)) ⋏ ~q ⟶ ⊥ := imply_left_remove_conj! (p := ~q) this;
-  have : 𝐆𝐋 ⊢! ⋀(Γ.remove (~q)) ⟶ ~q ⟶ ⊥ := and_imply_iff_imply_imply'!.mp this;
-  have : 𝐆𝐋 ⊢! ⋀(Γ.remove (~q)) ⟶ q := imp_trans''! this $ imp_trans''! (and₂'! neg_equiv!) dne!
-  have : 𝐆𝐋 ⊢! ⋀((Γ.remove (~q)).remove (□q)) ⋏ □q ⟶ q := imply_left_remove_conj! (p := □q) this;
-  have : 𝐆𝐋 ⊢! ⋀((Γ.remove (~q)).remove (□q)) ⟶ (□q ⟶ q) := and_imply_iff_imply_imply'!.mp this;
-  have : 𝐆𝐋 ⊢! □(⋀(Γ.remove (~q)).remove (□q)) ⟶ □(□q ⟶ q) := imply_box_distribute'! this;
-  have : 𝐆𝐋 ⊢! □(⋀(Γ.remove (~q)).remove (□q)) ⟶ □q := imp_trans''! this axiomL!;
-  have : 𝐆𝐋 ⊢! ⋀□'(Γ.remove (~q)).remove (□q) ⟶ □q := imp_trans''! collect_box_conj! this;
-  have : (□'(Γ.remove (~q)).remove (□q)) ⊢[𝐆𝐋]! □q := provable_iff.mpr this;
-  have : X.theory *⊢[𝐆𝐋]! □q := by
-    apply Context.provable_iff.mpr;
-    use (□'List.remove (□q) (List.remove (~q) Γ));
-    constructor;
-    . intro r hr; simp at hr;
-      obtain ⟨s, hs, es⟩ := hr; subst es;
-      have ⟨s_mem', hs₁⟩ := List.mem_remove_iff.mp hs;
-      have ⟨s_mem, hs₂⟩ := List.mem_remove_iff.mp s_mem';
-      clear hs s_mem';
-      have := hΓ₁ s s_mem;
-      simp at this;
-      rcases this with ((ns₁ | hs₂) | bs_mem | b);
-      . contradiction;
-      . contradiction;
-      . assumption;
-      . obtain ⟨t, ht, et⟩ := b; subst et;
-        apply membership_iff.mpr;
-        apply axiomFour'!;
-        apply membership_iff.mp;
-        assumption;
-    . assumption;
-  have : □q ∈ X.theory := membership_iff.mpr this;
-  contradiction;
-
-open Formula MaximalConsistentTheory in
-lemma GL_truthlemma
-  {p : Formula α} {X : (CanonicalModel 𝐆𝐋).World} {q : Formula α} (hq : q ∈ 𝒮 p) :
-  Satisfies (GLFilteredModel p) ⟦X⟧ q ↔ q ∈ X.theory := by
-  induction q using Formula.rec' generalizing X with
-  | hbox q ih =>
-    constructor;
-    . contrapose;
-      intro h;
-      obtain ⟨Y, hY⟩ := lindenbaum (Λ := 𝐆𝐋) (T := {□q, ~q} ∪ (□''⁻¹X.theory ∪ □''□''⁻¹X.theory)) $ GL_truthlemma.lemma1 h;
-      simp [Satisfies];
-      use ⟦Y⟧;
-      constructor;
-      . apply GLFilteredFrame.def_rel.mpr;
-        simp at hY;
-        have ⟨hY₁, ⟨hY₂, hY₃⟩⟩ := hY;
-        simp_all;
-        constructor;
-        . intro q _ bq_mem_X;
-          constructor;
-          . apply hY₂; simpa;
-          . apply hY₃; simpa;
-        . use q;
-          simp_all;
-          tauto;
-      . apply ih (by aesop) |>.not.mpr;
-        apply iff_mem_neg.mp;
-        apply hY;
-        simp;
-    . intro bq_mem_X QY RXY;
-      obtain ⟨Y, hY⟩ := Quotient.exists_rep QY; subst hY;
-      have ⟨h₁, _⟩ := GLFilteredFrame.def_rel.mp RXY; simp at h₁;
-      have ⟨q_mem_Y, _⟩ := h₁ q hq bq_mem_X;
-      exact ih (by aesop) |>.mpr q_mem_Y;
-  | _ =>
-    simp_all [Satisfies, StandardFilterationValuation];
-    try aesop;
-    done;
-
-lemma exists_finite_frame : ¬𝔽ꟳ# ⊧ p ↔ ∃ F ∈ 𝔽.toFiniteFrameClass, ¬F# ⊧ p := by
-  constructor;
-  . simp;
-  . rintro ⟨F, hF₁, hF₂⟩;
-    simp; use F;
-    constructor;
-    . simp_all;
-    . assumption;
-
-private lemma GL_completeAux {p : Formula α} : TransitiveIrreflexiveFrameClass.{u}ꟳ# ⊧ p → 𝐆𝐋 ⊢! p := by
-  contrapose;
-  intro h;
-  apply exists_finite_frame.mpr;
-  use (GLFilteredFrame p);
-  constructor;
-  . exact ⟨transitive_GLFilteredFrame, irreflexive_GLFilteredFrame⟩;
-  . simp [Formula.Kripke.ValidOnFrame, Formula.Kripke.ValidOnModel];
-    obtain ⟨X, hX⟩ := lindenbaum (Λ := 𝐆𝐋) (T := {~p}) (Theory.unprovable_iff_singleton_neg_consistent.mp h);
-    use (GLFilteredModel p).Valuation, ⟦X⟧;
-    apply GL_truthlemma (by simp) |>.not.mpr;
-    apply MaximalConsistentTheory.iff_mem_neg.mp;
-    simpa using hX;
-
-instance GL_complete : Complete (𝐆𝐋 : DeductionParameter α) TransitiveIrreflexiveFrameClass.{u}ꟳ# := ⟨GL_completeAux⟩
-
-instance : FiniteFrameProperty (α := α) 𝐆𝐋 TransitiveIrreflexiveFrameClass where
-
-end Completeness
-
-end Kripke
-
-end LO.Modal.Standard
+import Logic.Modal.Standard.Kripke.GL.Completeness
 
 -- TODO: Move to vorspiel or etc.
 namespace List
 
 variable {l l₁ l₂ : List α}
 variable {R : α → α → Prop}
-
--- TODO: 使っていない．Mathlibにこれに対応する補題があるかは微妙．
-lemma head?_eq_head_of_ne_nil (h : l₁ ≠ []) : l₁.head? = some (l₁.head h):= by
-  induction l₁ with
-  | nil => contradiction;
-  | cons => simp_all;
 
 lemma Chain'.nodup_of_trans_irreflex (R_trans : Transitive R) (R_irrefl : Irreflexive R) (h_chain : l.Chain' R) : l.Nodup := by
   by_contra hC;
@@ -618,6 +283,7 @@ instance : CoeSort (FiniteTransitiveTreeModel α) (Type u) := ⟨World⟩
 @[reducible]
 instance {M : FiniteTransitiveTreeModel α} : Semantics (Formula α) (M.World) := Formula.Kripke.Satisfies.semantics (M := M.toModel)
 
+
 end FiniteTransitiveTreeModel
 
 
@@ -632,7 +298,7 @@ variable {p : Formula α}
 
 open Classical
 
-lemma valid_on_FiniteTransitiveTreeClass_of_valid_on_TransitiveIrreflexiveFrameClass (h : TransitiveIrreflexiveFrameClass.{u}ꟳ# ⊧ p) : ∀ T : FiniteTransitiveTree.{u}, T# ⊧ p := by
+lemma valid_on_FiniteTransitiveTreeClass_of_valid_on_TransitiveIrreflexiveFrameClass (h : TransitiveIrreflexiveFrameClass.{v}ꟳ# ⊧ p) : ∀ T : FiniteTransitiveTree.{v}, T# ⊧ p := by
   simp at h;
   intro T;
   apply @h T.toFrame T.toFiniteFrame;
@@ -640,11 +306,11 @@ lemma valid_on_FiniteTransitiveTreeClass_of_valid_on_TransitiveIrreflexiveFrameC
   . exact T.rel_irreflexive;
   . tauto;
 
-lemma satisfies_at_root_on_FiniteTransitiveTree (h : ∀ F : FiniteTransitiveTree.{u}, F# ⊧ p) : ∀ M : FiniteTransitiveTreeModel.{u, u} α, Satisfies M.toModel M.root p := by
+lemma satisfies_at_root_on_FiniteTransitiveTree (h : ∀ F : FiniteTransitiveTree.{v}, F# ⊧ p) : ∀ M : FiniteTransitiveTreeModel.{u, v} α, Satisfies M.toModel M.root p := by
   intro M;
   exact h M.Tree M.Valuation M.root
 
-lemma valid_on_TransitiveIrreflexiveFrameClass_of_satisfies_at_root_on_FiniteTransitiveTree : (∀ M : FiniteTransitiveTreeModel.{u, u} α, Satisfies M.toModel M.root p) → TransitiveIrreflexiveFrameClass.{u}ꟳ# ⊧ p := by
+lemma valid_on_TransitiveIrreflexiveFrameClass_of_satisfies_at_root_on_FiniteTransitiveTree : (∀ M : FiniteTransitiveTreeModel.{u, v} α, Satisfies M.toModel M.root p) → TransitiveIrreflexiveFrameClass.{v}ꟳ# ⊧ p := by
   rintro H _ ⟨F, ⟨F_trans, F_irrefl⟩, rfl⟩ V r;
   let M : Kripke.Model α := ⟨F, V⟩;
   apply Model.PointGenerated.modal_equivalent_to_root M F_trans r |>.mp;
@@ -671,7 +337,6 @@ lemma iff_unprovable_GL_exists_unsatisfies_at_root_on_FiniteTransitiveTree : �
     apply iff_provable_GL_satisfies_at_root_on_FiniteTransitiveTree.mpr;
   . contrapose; simp;
     apply iff_provable_GL_satisfies_at_root_on_FiniteTransitiveTree.mp;
-
 
 end
 
@@ -767,7 +432,6 @@ end
 
 end Kripke
 
-
 section
 
 open System
@@ -823,6 +487,5 @@ noncomputable instance : System.Unnecessitation (𝐆𝐋 : DeductionParameter �
   unnec := λ h => GL_unnecessitation! ⟨h⟩ |>.some
 
 end
-
 
 end LO.Modal.Standard
